puzzled ... seem to have missed a file somehow

ulib/FStar.Buffer.fst
@@ -792,6 +792,16 @@ let to_seq #a b l =
   let i = v b.idx in
   Seq.slice s i (i + v l)
 
+
+// ocaml-only, used for conversions to Platform.bytes
+val to_seq_full: #a:Type -> b:buffer a -> ST (seq a)
+  (requires (fun h -> live h b))
+  (ensures  (fun h0 r h1 -> h0 == h1 /\ live h1 b /\ 
+			 r == as_seq #a h1 b ))
+let to_seq_full #a b =
+  let s = !b.content in
+  Seq.slice s i (i + v b.length)
+
 val index: #a:Type -> b:buffer a -> n:UInt32.t{v n < length b} -> Stack a
   (requires (fun h -> live h b))
   (ensures (fun h0 z h1 -> live h0 b /\ h1 == h0
